SP1Operations/Reader/JTypeReader.lean
@@ -1,2 +1,68 @@
 import SP1Operations.Reader.JTypeReader.Operation
 import SP1Operations.Reader.JTypeReader.Constraints
+
+namespace JTypeReader
+
+attribute [-simp] Opcode.trusted_instr
+
+-- iff-characterization of JTypeReader constraints
+lemma allHold_constraints_iff :
+  List.Forall SP1Constraint.toProp (constraints clk_high clk_low pc opcode instr_field_consts op_a_write_value cols is_real) ↔
+    (is_real = 0 ∨ is_real = 1) ∧
+    (¬is_real = 0 →
+      Opcode.trusted_instr (Opcode.ofNat opcode.val) cols.op_a
+        cols.op_b_imm[0] cols.op_b_imm[1] cols.op_b_imm[2] cols.op_b_imm[3]
+        cols.op_c_imm[0] cols.op_c_imm[1] cols.op_c_imm[2] cols.op_c_imm[3] 1 1 ∧
+      cols.op_a < 32 ∧
+      cols.op_b_imm[0] < 65536 ∧ cols.op_b_imm[1] < 65536 ∧ cols.op_b_imm[2] < 65536 ∧ cols.op_b_imm[3] < 65536 ∧
+      cols.op_c_imm[0] < 65536 ∧ cols.op_c_imm[1] < 65536 ∧ cols.op_c_imm[2] < 65536 ∧ cols.op_c_imm[3] < 65536 ∧
+      (cols.op_a_0 = 0 ∨ cols.op_a_0 = 1) ∧
+      (cols.op_a_0 = 1 ↔ cols.op_a = 0) ∧
+      pc[0] % 4 = 0 ∧
+      pc[0] < 65536 ∧ pc[1] < 65536 ∧ pc[2] < 65536 ∧
+      cols.op_a_memory.access_timestamp.diff_low_limb < 65536 ∧
+      (clk_low + 4 - cols.op_a_memory.access_timestamp.prev_low - 1 - cols.op_a_memory.access_timestamp.diff_low_limb) * 2130673921 < 256 ∧
+      Word.isU64 #v[cols.op_a_memory.prev_value[0], cols.op_a_memory.prev_value[1], cols.op_a_memory.prev_value[2], cols.op_a_memory.prev_value[3]]) ∧
+    (cols.op_a_0 ≠ 0 →
+      op_a_write_value[0] = 0 ∧
+      op_a_write_value[1] = 0 ∧
+      op_a_write_value[2] = 0 ∧
+      op_a_write_value[3] = 0)
+   := by
+    simp [constraints, sub_eq_zero, SP1Constraint.toProp, Fin.lt_def]
+    intros h_is_real
+    rcases h_is_real with h | h
+    · simp [h]
+      by_cases ha0 : cols.op_a_0 = 0
+      · simp [ha0]
+      · tauto
+    · simp [h]
+      by_cases hop_a_0 : cols.op_a_0 = 0
+      · simp [hop_a_0]
+        aesop
+      · simp [hop_a_0]
+        aesop
+
+lemma allHold_constraints_iff_is_real (h : is_real = 1) :
+  List.Forall SP1Constraint.toProp (constraints clk_high clk_low pc opcode instr_field_consts op_a_write_value cols is_real) ↔
+    Opcode.trusted_instr (Opcode.ofNat opcode.val) cols.op_a
+      cols.op_b_imm[0] cols.op_b_imm[1] cols.op_b_imm[2] cols.op_b_imm[3]
+      cols.op_c_imm[0] cols.op_c_imm[1] cols.op_c_imm[2] cols.op_c_imm[3] 1 1 ∧
+    cols.op_a < 32 ∧
+    cols.op_b_imm[0] < 65536 ∧ cols.op_b_imm[1] < 65536 ∧ cols.op_b_imm[2] < 65536 ∧ cols.op_b_imm[3] < 65536 ∧
+    cols.op_c_imm[0] < 65536 ∧ cols.op_c_imm[1] < 65536 ∧ cols.op_c_imm[2] < 65536 ∧ cols.op_c_imm[3] < 65536 ∧
+    (cols.op_a_0 = 0 ∨ cols.op_a_0 = 1) ∧
+    (cols.op_a_0 = 1 ↔ cols.op_a = 0) ∧
+    pc[0] % 4 = 0 ∧
+    pc[0] < 65536 ∧ pc[1] < 65536 ∧ pc[2] < 65536 ∧
+    cols.op_a_memory.access_timestamp.diff_low_limb < 65536 ∧
+    (clk_low + 4 - cols.op_a_memory.access_timestamp.prev_low - 1 - cols.op_a_memory.access_timestamp.diff_low_limb) * 2130673921 < 256 ∧
+    Word.isU64 #v[cols.op_a_memory.prev_value[0], cols.op_a_memory.prev_value[1], cols.op_a_memory.prev_value[2], cols.op_a_memory.prev_value[3]] ∧
+    (cols.op_a_0 ≠ 0 →
+      op_a_write_value[0] = 0 ∧
+      op_a_write_value[1] = 0 ∧
+      op_a_write_value[2] = 0 ∧
+      op_a_write_value[3] = 0)
+   := by aesop (add safe (by simp [allHold_constraints_iff]))
+
+end JTypeReader
